Renamings.

core/EvalExpressions.v
@@ -25,14 +25,14 @@ Definition evalIteratorExpr (r : Rule) (sm: SourceModel) (sp: list SourceElement
   | _ => 0
   end.
 
-Definition evalOutputPatternElementExpr (sm: SourceModel) (sp: list SourceElementType) (iter: nat) (o: OutputPatternElement)
+Definition evalOutputPatternElementExpr (o: OutputPatternUnit) (sm: SourceModel) (sp: list SourceElementType) (iter: nat) 
   : option TargetElementType := 
-  o.(ope_elementExpr) iter sm sp.
+  o.(opu_elementExpr) iter sm sp.
 
 Definition evalOutputPatternLinkExpr
-            (sm: SourceModel) (sp: list SourceElementType) (oe: TargetElementType) (iter: nat) (tr: list TraceLink)
-            (o: OutputPatternElement)
+            (sm: SourceModel) (sp: list SourceElementType) (oe: TargetElementType) (iter: nat) (tra: list TraceLink)
+            (o: OutputPatternUnit)
   : option (list TargetLinkType) :=
-  o.(ope_linkExpr) tr iter sm sp oe.
+  o.(opu_linkExpr) tra iter sm sp oe.
 
 End Expressions.
