core/Tactics.v
@@ -154,20 +154,20 @@ Ltac destruct_execute :=
   end.
 
 
-Ltac destruct_instantiatePattern H IN_MATCH_NEWNAME :=
+Ltac destruct_instantiateOnPattern H IN_MATCH_NEWNAME :=
   match type of H with 
-    In _ (instantiatePattern ?T _ _) =>
+    In _ (instantiateOnPattern ?T _ _) =>
       let e := fresh "r" in
-      rewrite (core.Certification.tr_instantiatePattern_in T) in H ;
+      rewrite (core.Certification.tr_instantiateOnPattern_in T) in H ;
       destruct H as [e [IN_MATCH_NEWNAME H]]
   end.
 
-Ltac destruct_instantiatePattern_auto :=
+Ltac destruct_instantiateOnPattern_auto :=
   match goal with 
-    [ H : In _ (instantiatePattern ?T _ _) |- _ ] =>
+    [ H : In _ (instantiateOnPattern ?T _ _) |- _ ] =>
       let H2 := fresh "IN_R" in
       let e := fresh "r" in
-      destruct_instantiatePattern H H2
+      destruct_instantiateOnPattern H H2
   end.
 
 
@@ -206,7 +206,7 @@ Ltac destruct_instantiateRuleOnPattern_auto :=
 Ltac destruct_instantiateIterationOnPattern H NEWNAME :=
   match type of H with 
     In _ (instantiateIterationOnPattern _ _ _ _) =>
-      let e := fresh "ope" in
+      let e := fresh "opu" in
       apply core.Certification.tr_instantiateIterationOnPattern_in in H ;
       destruct H as [e [NEWNAME H]]
   end.
@@ -232,15 +232,15 @@ Ltac unfold_instantiateElementOnPattern_auto :=
 
 Ltac destruct_apply_pattern H IN_MATCH_NEWNAME :=
   match type of H with 
-    In _ (applyPattern _ _ _) => 
+    In _ (applyOnPattern _ _ _) => 
       let R := fresh "r" in
-      apply core.Certification.tr_applyPattern_in in H ; 
+      apply core.Certification.tr_applyOnPattern_in in H ; 
       destruct H as (R & (IN_MATCH_NEWNAME & H))
 end.
 
 Ltac destruct_apply_pattern_auto :=
   match goal with 
-    [ H : In _ (applyPattern _ _ _) |- _ ] => 
+    [ H : In _ (applyOnPattern _ _ _) |- _ ] => 
       let IN1 := fresh "IN_MATCH" in
       destruct_apply_pattern H IN1
 end.
@@ -288,15 +288,15 @@ Ltac destruct_trace H :=
   | _ => fail "Failure in destruct_trace."
   end.
 
-Ltac destruct_tracePattern H :=
+Ltac destruct_traceOnPattern H :=
   match type of H with 
-    | In _ (tracePattern _ _ _) => 
+    | In _ (traceOnPattern _ _ _) => 
         let p:= fresh "r" in
         let IN := fresh "IN" in
-        unfold tracePattern in H ;
+        unfold traceOnPattern in H ;
         apply in_flat_map in H ; 
         destruct H as (p & (IN & H))
-  | _ => fail "Failure in destruct_tracePattern."
+  | _ => fail "Failure in destruct_traceOnPattern."
   end.
 
 
@@ -343,21 +343,21 @@ Lemma destruct_in_trace_lem {MM1 : Metamodel} {T1} {T2} {BEQ1} {BEQ2} :
     {t: Syntax.Transformation (tc:=Build_TransformationConfiguration MM1 (Build_Metamodel T1 T2 BEQ1 BEQ2))} 
   {cm} {l},
   In l (trace t cm) ->
-  exists p r i e te,   
+  exists p r i outpat te,   
     In p (allTuples t cm)
     /\ In r (Syntax.rules t) 
     /\ EvalExpressions.evalGuardExpr r cm p = true 
     /\ In i (seq 0 (EvalExpressions.evalIteratorExpr r cm p))
-    /\ In e (Syntax.r_outputPattern r)
+    /\ In outpat (Syntax.r_outputPattern r)
     /\ l = {|
-             TraceLink.source := (p, i, Syntax.ope_name e);
+             TraceLink.source := (p, i, Syntax.opu_name outpat);
              TraceLink.target := te
            |} 
-    /\ EvalExpressions.evalOutputPatternElementExpr cm p i e = return te .
+    /\ EvalExpressions.evalOutputPatternElementExpr outpat cm p i = return te .
 Proof.
   intros.
   destruct_trace H ; 
-  destruct_tracePattern H ; 
+  destruct_traceOnPattern H ; 
   destruct_traceRuleOnPattern H ; 
   destruct_traceIterationOnPattern H ; 
   destruct_in_optionToList H.
@@ -411,7 +411,7 @@ Proof.
   unfold modelElements.
 
   
-  unfold instantiatePattern.
+  unfold instantiateOnPattern.
   apply in_flat_map.
   exists se ; split ; [ exact IN_SOURCE | ].
 
@@ -438,7 +438,7 @@ Qed.
 Ltac destruct_any := 
   first [ 
       destruct_execute 
-    | destruct_instantiatePattern_auto 
+    | destruct_instantiateOnPattern_auto 
     | destruct_in_matchingRules_auto 
     | destruct_instantiateRuleOnPattern_auto 
     | destruct_instantiateIterationOnPattern_auto 
@@ -456,18 +456,18 @@ Lemma destruct_in_modelElements_execute_lem {MM1} {T1} {T2} {BEQ1} {BEQ2} :
     
   In a
     (modelElements (execute t cm)) ->
-  exists r sp n0 ope,
+  exists r sp n0 opu,
     In sp (allTuples t cm)
     /\ In r (Syntax.rules t) 
     /\ EvalExpressions.evalGuardExpr r cm sp = true 
     /\ In n0 (seq 0 (EvalExpressions.evalIteratorExpr r cm sp))
-    /\ In ope (Syntax.r_outputPattern r) 
-    /\ EvalExpressions.evalOutputPatternElementExpr cm sp n0 ope =
+    /\ In opu (Syntax.r_outputPattern r) 
+    /\ EvalExpressions.evalOutputPatternElementExpr opu cm sp n0 =
          return a.
 Proof.
   intros. 
   destruct_in_modelElements_execute H.  
-  destruct_instantiatePattern H NEW1. 
+  destruct_instantiateOnPattern H NEW1. 
   destruct_instantiateRuleOnPattern H NEW2. 
   destruct_instantiateIterationOnPattern H NEW3. 
   unfold_instantiateElementOnPattern H. 
@@ -488,7 +488,7 @@ Lemma destruct_in_modelLinks_execute_lem {MM1} {T1} {T2} {BEQ1} {BEQ2} :
       /\ EvalExpressions.evalGuardExpr r m sp = true
       /\ In n (seq 0 (EvalExpressions.evalIteratorExpr r m sp))
       /\ In p (Syntax.r_outputPattern r) 
-      /\ EvalExpressions.evalOutputPatternElementExpr m sp n p =
+      /\ EvalExpressions.evalOutputPatternElementExpr p m sp n =
          return te
   
   /\ EvalExpressions.evalOutputPatternLinkExpr m sp te n (trace t m) p = return tls
@@ -501,7 +501,7 @@ Proof.
   destruct_applyRuleOnPattern H IN_IT IN_APP_PAT. 
   destruct_applyIterationOnPattern IN_APP_PAT H_IN_OUTPAT.   
   destruct_in_matchingRules IN_RULE H_MATCH_RULE.
-  unfold applyElementOnPattern in IN_APP_PAT.
+  unfold applyUnitOnPattern in IN_APP_PAT.
   PropUtils.destruct_match IN_APP_PAT ; [ | ListUtils.unfold_In_cons IN_APP_PAT ].
   ListUtils.destruct_in_optionListToList IN_APP_PAT.
   eauto 15.
@@ -513,7 +513,7 @@ Ltac simpl_accessors_any H :=
         | ConcreteSyntax.simpl_elem_accessors H 
         | ConcreteSyntax.simpl_link_accessors H
         | Syntax.simpl_r_accessors H 
-        | Syntax.simpl_ope_accessors H]. 
+        | Syntax.simpl_opu_accessors H]. 
 
 Ltac progress_in_In_rules H :=
   match type of H with 
@@ -527,8 +527,8 @@ Ltac progress_in_In_rules H :=
 Ltac exploit_evaloutpat H :=
   match type of H with 
 
-  | EvalExpressions.evalOutputPatternElementExpr _ _ _ (Parser.parseOutputPatternElement _) = Some _ =>
-      unfold Parser.parseOutputPatternElement in H ;
+  | EvalExpressions.evalOutputPatternElementExpr _ _ _ (Parser.parseOutputPatternUnit _) = Some _ =>
+      unfold Parser.parseOutputPatternUnit in H ;
       exploit_evaloutpat H (* recursion *)
        
   | EvalExpressions.evalOutputPatternElementExpr _ _ _ _ = Some _ =>
@@ -559,12 +559,12 @@ Ltac progress_in_In_outpat H :=
         unfold_parseRule H ;
         progress_in_In_outpat H (* recursion *)
                       
-    | In ?ope (Syntax.r_outputPattern (Syntax.buildRule _ _ _ _)) =>
+    | In ?opu (Syntax.r_outputPattern (Syntax.buildRule _ _ _ _)) =>
         unfold Syntax.r_outputPattern in H ; 
         unfold ConcreteSyntax.r_outpat in H ;
         unfold List.map in H ;
         progress repeat unfold_In_cons H ;
-        subst ope 
+        subst opu 
             
   end.
 
@@ -613,7 +613,7 @@ Ltac destruct_in_trace_G :=
 
 Lemma transform_elements_fw {tc} cm p tp (t:Syntax.Transformation (tc:=tc)) :
   In p (allTuples t cm) ->
-  In tp (instantiatePattern t cm p) ->
+  In tp (instantiateOnPattern t cm p) ->
   In tp (modelElements (execute t cm)).
 Proof.
   intros IN1 IN2.
@@ -626,7 +626,7 @@ Qed.
 Lemma transform_element_fw {tc} cm e te (t:Syntax.Transformation (tc:=tc)) :
   0 < Syntax.arity t ->
   In e (modelElements cm) ->
-  In te (instantiatePattern t cm [e]) ->
+  In te (instantiateOnPattern t cm [e]) ->
   In te (modelElements (execute t cm)).
 Proof.
   intros A IN1 IN2.
