transformations/Class2Relational/C2RTactics.v
@@ -61,7 +61,7 @@ Ltac unfold_toEData H :=
 
 Lemma transform_element_fw cm e te :
   In e (modelElements cm) ->
-  In te (instantiatePattern Class2Relational cm [e]) ->
+  In te (instantiateOnPattern Class2Relational cm [e]) ->
   In te (modelElements (execute Class2Relational cm)).
 Proof.
   intros IN1 IN2.
